coq/proof/SimulationNop.v
@@ -1,0 +1,401 @@
+Require Import syntax.
+Require Import alist.
+Require Import FMapWeakList.
+
+Require Import Classical.
+Require Import Coqlib.
+Require Import infrastructure.
+Require Import Metatheory.
+Import LLVMsyntax.
+Import LLVMinfra.
+Require Import opsem.
+
+Require Import sflib.
+Require Import paco.
+Import Opsem.
+
+Require Import TODO.
+Require Import GenericValues.
+Require Import MemInv.
+Require Import Nop.
+Require Import SimulationLocal.
+
+Definition LOCALS_TODO: Prop. Admitted.
+Definition ALLOCAS_TODO: Prop. Admitted.
+Definition MEM_TODO: Prop. Admitted.
+Definition CONF_TODO: Prop. Admitted.
+
+Inductive nop_state_sim
+          (conf_src conf_tgt:Config)
+          (stack0_src stack0_tgt:ECStack)
+          (inv:Relational.t):
+  forall (idx:nat) (st_src st_tgt:State), Prop :=
+| nop_state_sim_intro
+    fdef_src fdef_tgt
+    l s_src s_tgt
+    cmds_src cmds_tgt term locals_src locals_tgt allocas_src allocas_tgt
+    mem_src mem_tgt
+    (FDEF: nop_fdef fdef_src fdef_tgt)
+    (CMDS: nop_cmds cmds_src cmds_tgt)
+    (LOCALS: LOCALS_TODO)
+    (ALLOCAS: ALLOCAS_TODO)
+    (MEM: Relational.sem conf_src conf_tgt mem_src mem_tgt inv):
+    nop_state_sim
+      conf_src conf_tgt
+      stack0_src stack0_tgt inv
+      (length cmds_tgt)
+      (mkState
+         (mkEC fdef_src (l, s_src) cmds_src term locals_src allocas_src)
+         stack0_src
+         mem_src)
+      (mkState
+         (mkEC fdef_tgt (l, s_tgt) cmds_tgt term locals_tgt allocas_tgt)
+         stack0_tgt
+         mem_tgt)
+.
+
+Lemma locals_init
+      inv la gvs_tgt
+    args_src args_tgt
+    conf_src conf_tgt
+    (CONF: CONF_TODO)
+    (ARGS: list_forall2 (GVs.inject inv.(Relational.inject)) args_src args_tgt)
+    (LOCALS : initLocals (CurTargetData conf_tgt) la args_tgt = Some gvs_tgt) :
+  initLocals (CurTargetData conf_src) la args_src =
+  initLocals (CurTargetData conf_tgt) la args_tgt.
+Proof.
+Admitted.
+
+Lemma nop_init
+      conf_src conf_tgt
+      stack0_src stack0_tgt
+      header
+      blocks_src blocks_tgt
+      args_src args_tgt
+      mem_src mem_tgt
+      inv
+      ec_tgt
+      (NOP_FDEF: nop_fdef (fdef_intro header blocks_src)
+                          (fdef_intro header blocks_tgt))
+      (NOP_FIRST_MATCHES: option_map fst (hd_error blocks_src) = option_map fst (hd_error blocks_tgt))
+      (ARGS: list_forall2 (GVs.inject inv.(Relational.inject)) args_src args_tgt)
+      (MEM: MEM_TODO)
+      (CONF: CONF_TODO)
+      (INIT: init_fdef conf_tgt (fdef_intro header blocks_tgt) args_tgt ec_tgt):
+  exists ec_src idx,
+    init_fdef conf_src (fdef_intro header blocks_src) args_src ec_src /\
+    nop_state_sim
+      conf_src conf_tgt
+      stack0_src stack0_tgt
+      inv idx
+      (mkState ec_src stack0_src mem_src)
+      (mkState ec_tgt stack0_tgt mem_tgt).
+Proof.
+  inv INIT. inv NOP_FDEF. inv FDEF.
+  destruct blocks_src, lb; inv NOP_FIRST_MATCHES; try inv ENTRY.
+  destruct b. ss. subst. destruct s.
+  esplits.
+  - econs; ss. rewrite <- LOCALS. eapply locals_init; eauto.
+  - generalize (BLOCKS l'). intro B. ss.
+    destruct (_ == _) in B; [|done].
+    ss. des. subst.
+    econs; eauto.
+    + econs; eauto.
+    + admit.
+    + admit.
+Admitted.
+
+Inductive status :=
+| status_call
+| status_return
+| status_return_void
+| status_step
+.
+
+(* TODO *)
+Definition get_status (ec:ExecutionContext): status :=
+  match ec.(CurCmds) with
+  | c::_ =>
+    match c with
+    | insn_call _ _ _ _ _ _ _ => status_call
+    | _ => status_step
+    end
+  | nil =>
+    match ec.(Terminator) with
+    | insn_return _ _ _ => status_return
+    | insn_return_void _ => status_return_void
+    | _ => status_step
+    end
+  end.
+
+Lemma get_status_call_inv ec
+      (CALL: get_status ec = status_call):
+  exists id noret attrs ty varg f args cmds,
+    ec.(CurCmds) = (insn_call id noret attrs ty varg f args)::cmds.
+Proof.
+  unfold get_status in *. destruct ec. ss.
+  destruct CurCmds0; ss.
+  - destruct Terminator0; ss.
+  - destruct c; ss.
+    esplits; eauto.
+Qed.
+
+Lemma get_status_return_inv ec
+      (CALL: get_status ec = status_return):
+    ec.(CurCmds) = [] /\
+    exists id typ value, ec.(Terminator) = insn_return id typ value.
+Proof.
+  unfold get_status in *. destruct ec. ss. destruct CurCmds0.
+  - destruct Terminator0; ss. esplits; ss.
+  - destruct c; ss.
+Qed.
+
+Lemma get_status_return_void_inv ec
+      (CALL: get_status ec = status_return_void):
+    ec.(CurCmds) = [] /\
+    exists id, ec.(Terminator) = insn_return_void id.
+Proof.
+  unfold get_status in *. destruct ec. ss. destruct CurCmds0.
+  - destruct Terminator0; ss. esplits; ss.
+  - destruct c; ss.
+Qed.
+
+(* TODO
+ - tgt cmds =           [non-nop] ++ .. =>
+   src cmds = [nops] ++ [non-nop] ++ .. & src, tgt related
+ - tgt cmds = [nop] ++ ..(A) =>
+    + tgt proceeds, src waits
+    + index decr by 1
+    + src cmds & A related
+ *)
+
+Lemma nop_step:
+  nop_state_sim <8= sim_local.
+Proof.
+  intros conf_src conf_tgt stack0_src stack0_tgt.
+  pcofix CIH.
+  intros inv0 idx0 st_src st_tgt SIM. pfold.
+  generalize (classic (stuck_state conf_tgt st_tgt)). intro STUCK. des.
+  { inv SIM. eapply _sim_local_error.
+    - econs 1.
+    - admit. (* tgt stuck -> src stuck *)
+  }
+  destruct st_src as [ec_src ecs_src mem_src].
+  destruct st_tgt as [ec_tgt ecs_tgt mem_tgt].
+  destruct (get_status ec_tgt) eqn:TGT.
+  - (* call *)
+    exploit get_status_call_inv; eauto. i. des.
+    inv SIM. ss. subst.
+    eapply _sim_local_call.
+    + econs 1.
+    + ss.
+
+admit.
+  - (* return *)
+    admit.
+  - (* return_void *)
+    admit.
+  - (* step *)
+    admit.
+
+(* inv EC_INJECT. simpl in *. subst. *)
+(*     apply get_status_call_inv in TGT. des. simpl in *. subst. *)
+(*     exploit identity_step_call_function; ii; eauto. *)
+(*     des. *)
+(*     exploit identity_step_call_parameter; ii; eauto. *)
+(*     des. *)
+(*     eapply _sim_local_call; *)
+(*       repeat (simpl in *; eauto). *)
+(*     + i. eexists. right. apply CIH. *)
+(*       econs; simpl; eauto. *)
+(*       econs; eauto. *)
+(*   - *)
+(*     inv EC_INJECT; simpl in *; auto. *)
+(*     symmetry in H, H0. simpl in *; subst. *)
+(*     eapply get_status_return_inv in TGT. des. simpl in *. *)
+(*     exploit identity_step_return; eauto; ii; des; subst. *)
+(*     eapply _sim_local_return; repeat (simpl in *; eauto). *)
+(*     + admit. *)
+(*   - inv EC_INJECT. *)
+(*     symmetry in H. symmetry in H0. *)
+(*     simpl in *; subst. *)
+(*     eapply get_status_return_void_inv in TGT; des. *)
+(*     eapply _sim_local_return_void; repeat (simpl in *; eauto). *)
+(*   - *)
+(*     destruct conf_src. *)
+(*     eapply _sim_local_step; simpl in *; eauto. *)
+(*     ii. *)
+(*     do 5 eexists. *)
+(*     splits. *)
+(*     + econs. *)
+(*     + admit. *)
+(*       (* destruct event. *) *)
+(*       (* * eapply sInsn_stutter. admit. *) *)
+(*       (* * *) *)
+(*       (*   econs; eauto. *) *)
+(*       (*   inv EC_INJECT. *) *)
+(*       (*   econs. *) *)
+(*       (*   instantiate (1:=inv0). admit. *) *)
+
+(*       (*   unfold stuck_state, not in NO_ERROR. *) *)
+(*       (*   apply double_neg in NO_ERROR. *) *)
+(*     + instantiate (1:=inv0). *)
+(*       admit. *)
+(*     + right. apply CIH. *)
+(*       econs; simpl; eauto. *)
+(*       instantiate (2:=mkState ec_src ecs_src mem_src). *)
+(*       instantiate (1:=mkState ec_tgt ecs_tgt mem_tgt). *)
+(*       admit. *)
+(*       simpl; auto. *)
+(*       simpl; auto. *)
+(*       inv STEP; simpl; auto; inv TGT. *)
+(*   Unshelve. *)
+(*   apply {| *)
+(*       CurFunction := fdef0; *)
+(*       CurBB := block0; *)
+(*       CurCmds := cmds0; *)
+(*       Terminator := terminator0; *)
+(*       Locals := locals2; *)
+(*       Allocas := allocas2 |}. *)
+
+    (* { *)
+    (* destruct conf_src. *)
+    (* eapply _sim_local_step; simpl in *; eauto. *)
+    (* unfold stuck_state, not. *)
+    (* apply double_neg2. *)
+    (* + (* ERROR should imply it *) admit. *)
+    (* + i. eexists _, _, st3_tgt, _, _. splits; simpl in *; eauto. *)
+    (*   * econs; eauto. *)
+    (*     inv EC_INJECT. *)
+    (*     (* destruct cmds0, terminator0; simpl in *; inv TGT. *) *)
+    (*     admit. *)
+    (*   * instantiate (1:=inv0). admit. *)
+    (*   * right. apply CIH. *)
+    (*     econs; simpl; eauto. *)
+    (*     instantiate (1:=mkState ec_src ecs_src mem_src). *)
+    (*     admit. *)
+    (*     simpl; auto. *)
+    (*     inv STEP; simpl; auto; inv TGT. *)
+    (* } *)
+Admitted.
+
+Lemma nop_sim
+      conf_src conf_tgt
+      header
+      blocks_src blocks_tgt
+      (NOP: nop_fdef (fdef_intro header blocks_src) (fdef_intro header blocks_tgt))
+      (NOP_FIRST_MATCHES: option_map fst (hd_error blocks_src) = option_map fst (hd_error blocks_tgt)):
+  sim_func conf_src conf_tgt (fdef_intro header blocks_src) (fdef_intro header blocks_tgt).
+Proof.
+  ii.
+  exploit nop_init; eauto.
+  { admit. }
+  { admit. }
+  i. des.
+  esplits; eauto.
+  apply nop_step. eauto.
+Admitted.
+
+Lemma identity_step_call_function
+      conf_src conf_tgt mem_src mem_tgt inv
+      CurTargetData
+      locals_tgt locals_src
+      allocas_tgt
+      fdef_tgt block_tgt
+      ecs_tgt
+      id noret attrs ty varg f args
+      cmds terminator
+      (LOCALS : LOCALS_TODO)
+      (ALLOCAS : ALLOCAS_TODO)
+      (MEM_INJECT : Relational.sem conf_src conf_tgt mem_src mem_tgt inv)
+      (NO_ERROR :
+         ~(stuck_state
+             conf_tgt
+             {|
+               EC := {|
+                  CurFunction := fdef_tgt;
+                  CurBB := block_tgt;
+                  CurCmds := insn_call id noret attrs ty varg f args
+                             :: cmds;
+                  Terminator := terminator;
+                  Locals := locals_tgt;
+                  Allocas := allocas_tgt |};
+            ECS := ecs_tgt;
+            Mem := mem_tgt |})):
+  exists funval_src funval_tgt,
+    getOperandValue (CurTargetData conf_tgt) f locals_tgt
+                    (Globals conf_tgt) = Some funval_tgt /\
+     getOperandValue (CurTargetData conf_src) f locals_src
+                    (Globals conf_src) = Some funval_src /\
+     GVs.inject (Relational.inject inv) funval_src funval_tgt.
+Proof.
+Admitted.
+
+Lemma identity_step_call_parameter
+      conf_src conf_tgt mem_src mem_tgt inv
+      CurTargetData
+      locals_tgt locals_src
+      allocas_tgt
+      fdef_tgt block_tgt
+      ecs_tgt
+      id noret attrs ty varg f args
+      cmds terminator
+      (LOCALS : True)
+      (ALLOCAS : True)
+      (MEM_INJECT : Relational.sem conf_src conf_tgt mem_src mem_tgt inv)
+      (NO_ERROR :
+         ~(stuck_state
+             conf_tgt
+             {|
+               EC := {|
+                      CurFunction := fdef_tgt;
+                      CurBB := block_tgt;
+                      CurCmds := insn_call id noret attrs ty varg f args
+                                           :: cmds;
+                      Terminator := terminator;
+                      Locals := locals_tgt;
+                      Allocas := allocas_tgt |};
+               ECS := ecs_tgt;
+               Mem := mem_tgt |})):
+  exists args_src args_tgt,
+    params2GVs (CurTargetData conf_src) args locals_src (Globals conf_src) =
+    Some args_src /\
+    params2GVs (CurTargetData conf_tgt) args locals_tgt (Globals conf_tgt) =
+    Some args_tgt /\
+    list_forall2 (GVs.inject (Relational.inject inv)) args_src args_tgt.
+  Admitted.
+
+Lemma identity_step_return
+      inv
+      mem_src conf_src
+      ecs_tgt mem_tgt conf_tgt
+      (* (fdef_src : fdef) *)
+      (* (block_src : blocks) *)
+      (* cmds_src terminator_src locals_src allocas_src *)
+      fdef_tgt block_tgt cmds_tgt terminator_tgt locals_tgt allocas_tgt
+      ec_src
+      id typ value
+      (MEM_INJECT : Relational.sem conf_src conf_tgt mem_src mem_tgt inv)
+      (LOCALS : True)
+      (ALLOCALS : True)
+      (NO_ERROR :
+         ~(stuck_state
+             conf_tgt
+             {|
+               EC := {|
+                      CurFunction := fdef_tgt;
+                      CurBB := block_tgt;
+                      CurCmds := cmds_tgt;
+                      Terminator := terminator_tgt;
+                      Locals := locals_tgt;
+                      Allocas := allocas_tgt |};
+               ECS := ecs_tgt;
+               Mem := mem_tgt |}))
+      (TGT : terminator_tgt = insn_return id typ value):
+  exists retval_src retval_tgt,
+    getOperandValue (CurTargetData conf_src) value (Locals ec_src)
+                    (Globals conf_src) = Some retval_src /\
+    getOperandValue (CurTargetData conf_tgt) value locals_tgt
+                    (Globals conf_tgt) = Some retval_tgt /\
+    GVs.inject (Relational.inject inv) retval_src retval_tgt.
+  Admitted.
